theories/simplang/notation.v
@@ -7,30 +7,21 @@ Coercion LitInt : Z >-> base_lit.
 Coercion LitBool : bool >-> base_lit.
 Coercion LitLoc : loc >-> base_lit.
 
-Coercion App : expr >-> Funclass.
-
 Coercion Val : val >-> expr.
 Coercion Var : string >-> expr.
 
 (** Define some derived forms. *)
-Notation Lam x e := (Rec BAnon x e) (only parsing).
-Notation Let x e1 e2 := (App (Lam x e2) e1) (only parsing).
 Notation Seq e1 e2 := (Let BAnon e1 e2) (only parsing).
-Notation LamV x e := (RecV BAnon x e) (only parsing).
-Notation LetCtx x e2 := (AppRCtx (LamV x e2)) (only parsing).
 Notation SeqCtx e2 := (LetCtx BAnon e2) (only parsing).
-Notation Match e0 x1 e1 x2 e2 := (Case e0 (Lam x1 e1) (Lam x2 e2)) (only parsing).
 Notation Alloc e := (AllocN (Val $ LitV $ LitInt 1) e) (only parsing).
 (** Compare-and-set (CAS) returns just a boolean indicating success or failure. *)
 Notation CAS l e1 e2 := (Snd (CmpXchg l e1 e2)) (only parsing).
 
-(* Skip should be atomic, we sometimes open invariants around
-   it. Hence, we need to explicitly use LamV instead of e.g., Seq. *)
-Notation Skip := (App (Val $ LamV BAnon (Val $ LitV LitUnit)) (Val $ LitV LitUnit)).
-
 (* No scope for the values, does not conflict and scope is often not inferred
 properly. *)
 Notation "# l" := (LitV l%Z%V%stdpp) (at level 8, format "# l").
+(* to avoid collisions with binders *)
+Notation "#f l" := (LitV (LitFn l%stdpp)) (at level 8, format "#f l").
 
 (** Syntax inspired by Coq/Ocaml. Constructions with higher precedence come
     first. *)
@@ -90,48 +81,20 @@ Notation "~ e" := (UnOp NegOp e%E) (at level 75, right associativity) : expr_sco
 (* The unicode ← is already part of the notation "_ ← _; _" for bind. *)
 Notation "e1 <- e2" := (Store e1%E e2%E) (at level 80) : expr_scope.
 
-(* The breaking point '/  ' makes sure that the body of the rec is indented
-by two spaces in case the whole rec does not fit on a single line. *)
-Notation "'rec:' f x := e" := (Rec f%binder x%binder e%E)
-  (at level 200, f at level 1, x at level 1, e at level 200,
-   format "'[' 'rec:'  f  x  :=  '/  ' e ']'") : expr_scope.
-Notation "'rec:' f x := e" := (RecV f%binder x%binder e%E)
-  (at level 200, f at level 1, x at level 1, e at level 200,
-   format "'[' 'rec:'  f  x  :=  '/  ' e ']'") : val_scope.
 Notation "'if:' e1 'then' e2 'else' e3" := (If e1%E e2%E e3%E)
   (at level 200, e1, e2, e3 at level 200) : expr_scope.
 
-(** Derived notions, in order of declaration. The notations for let and seq
-are stated explicitly instead of relying on the Notations Let and Seq as
-defined above. This is needed because App is now a coercion, and these
-notations are otherwise not pretty printed back accordingly. *)
-Notation "'rec:' f x y .. z := e" := (Rec f%binder x%binder (Lam y%binder .. (Lam z%binder e%E) ..))
-  (at level 200, f, x, y, z at level 1, e at level 200,
-   format "'[' 'rec:'  f  x  y  ..  z  :=  '/  ' e ']'") : expr_scope.
-Notation "'rec:' f x y .. z := e" := (RecV f%binder x%binder (Lam y%binder .. (Lam z%binder e%E) ..))
-  (at level 200, f, x, y, z at level 1, e at level 200,
-   format "'[' 'rec:'  f  x  y  ..  z  :=  '/  ' e ']'") : val_scope.
-
 (* The breaking point '/  ' makes sure that the body of the λ: is indented
 by two spaces in case the whole λ: does not fit on a single line. *)
-Notation "λ: x , e" := (Lam x%binder e%E)
+(* Note: this is a context for use with the function call mechanism of SimpLang. *)
+Notation "λ: x , e" := ([LetCtx x%binder e%E])
   (at level 200, x at level 1, e at level 200,
    format "'[' 'λ:'  x ,  '/  ' e ']'") : expr_scope.
-Notation "λ: x y .. z , e" := (Lam x%binder (Lam y%binder .. (Lam z%binder e%E) ..))
-  (at level 200, x, y, z at level 1, e at level 200,
-   format "'[' 'λ:'  x  y  ..  z ,  '/  ' e ']'") : expr_scope.
 
-Notation "λ: x , e" := (LamV x%binder e%E)
-  (at level 200, x at level 1, e at level 200,
-   format "'[' 'λ:'  x ,  '/  ' e ']'") : val_scope.
-Notation "λ: x y .. z , e" := (LamV x%binder (Lam y%binder .. (Lam z%binder e%E) .. ))
-  (at level 200, x, y, z at level 1, e at level 200,
-   format "'[' 'λ:'  x  y  ..  z ,  '/  ' e ']'") : val_scope.
-
-Notation "'let:' x := e1 'in' e2" := (Lam x%binder e2%E e1%E)
+Notation "'let:' x := e1 'in' e2" := (Let x%binder e1%E e2%E)
   (at level 200, x at level 1, e1, e2 at level 200,
    format "'[' 'let:'  x  :=  '[' e1 ']'  'in'  '/' e2 ']'") : expr_scope.
-Notation "e1 ;; e2" := (Lam BAnon e2%E e1%E)
+Notation "e1 ;; e2" := (Let BAnon e1%E e2%E)
   (at level 100, e2 at level 200,
    format "'[' '[hv' '[' e1 ']' ;;  ']' '/' e2 ']'") : expr_scope.
 
